@@ -1,0 +1,10 @@
+/-
+`filedup` meets its specification, given `acquire` and `release`.
+-/
+import Xv6.ProofFiledup
+
+namespace Xv6
+
+theorem Filedup (AC : ACQUIRE) (RE : RELEASE) : FILEDUP := filedup_proof AC RE
+
+end Xv6
